merge

MoreNorm.v
@@ -1,6 +1,74 @@
-From Lambda Require Import Map.
+Require Import Bool.Bool.
+Require Import Classes.CEquivalence.
+Require Classes.CMorphisms.
+From Lambda Require Import LibTactics.
 Set Default Goal Selector "!".
 
+Section STLC.
+
+(* Map *)
+Variable INDEX : Type.
+Variable eqb : INDEX -> INDEX -> bool.
+Infix "=?" := eqb (at level 70).
+Variable eqb_spec : forall x y, reflect (x=y) (x=?y).
+
+Property eqb_refl x : (x =? x) = true.
+Proof. destruct (eqb_spec x x); auto. Defined.
+Property eqb_eq x y : (x =? y) = true <-> x = y.
+Proof. destruct (eqb_spec x y); split; auto. congruence. Defined.
+Property eqb_neq x y : (x =? y) = false <-> x <> y.
+Proof. destruct (eqb_spec x y); split; auto; congruence. Defined.
+Hint Resolve eqb_eq eqb_neq : core.
+
+Definition map (A : Type) : Type := INDEX -> option A.
+Definition empty {A : Type} : map A := fun _ => None.
+Definition update {A : Type} x v : map A -> map A :=
+  fun m x' => if x =? x' then Some v else m x'.
+Notation "x '|->' v ';' m" := (update x v m) (at level 100, v at next level, right associativity).
+Notation "x '|->' v" := (update x v empty) (at level 100).
+
+Property update_eq A (m : map A) x v : (x |-> v ; m) x = Some v.
+Proof. repeat unfolds; rewrite eqb_refl; reflexivity. Defined.
+Property update_neq A (m : map A) x1 x2 v :
+  x2 <> x1 -> (x2 |-> v ; m) x1 = m x1.
+Proof. intros Hneq. repeat unfolds. rewrite <- eqb_neq in Hneq. rewrite Hneq. reflexivity. Defined.
+
+Definition mapeq {A} (m1 m2 : map A) : Type := forall x, m1 x = m2 x.
+Notation "f ~ g" := (mapeq f g) (at level 70).
+Fact eq_to_mapeq {A} (f g : map A) : f = g -> f ~ g.
+Proof. congruence. Defined.
+Fact mapeq_refl {A} (f : map A) : f ~ f.
+Proof. congruence. Defined.
+Fact mapeq_sym {A} (f g : map A) : f ~ g -> g ~ f.
+Proof. congruence. Defined.
+Fact mapeq_trans {A} (f g h : map A) : f ~ g -> g ~ h -> f ~ h.
+Proof. congruence. Defined.
+Fact mapeq_cong {A} (f g : map A) x v :
+  f ~ g -> (x |-> v; f) ~ (x |-> v; g).
+Proof. intros H x0. repeat unfolds. destruct (x =? x0); auto. Defined.
+Hint Resolve eq_to_mapeq mapeq_refl mapeq_sym : core.
+
+Property update_shadow A (m : map A) x v1 v2 :
+  (x |-> v2 ; x |-> v1 ; m) ~ (x |-> v2 ; m).
+Proof. intros x0; repeat unfolds; destruct (x =? x0); reflexivity. Defined.
+Property update_permute A (m : map A) x1 x2 v1 v2 :
+  x1 <> x2 -> (x1 |-> v1 ; x2 |-> v2 ; m) ~ (x2 |-> v2 ; x1 |-> v1 ; m).
+Proof. intros Hneq x; repeat unfolds; destruct (eqb_spec x1 x), (eqb_spec x2 x); auto; congruence. Defined.
+
+Definition includedin {A} (m m' : map A) :=
+  forall x v, m x = Some v -> m' x = Some v.
+Property includedin_update A (m m' : map A) (x : INDEX) (vx : A) :
+  includedin m m' ->
+  includedin (x |-> vx ; m) (x |-> vx ; m').
+Proof.
+  unfold includedin.
+  intros H y vy.
+  destruct (eqb_spec x y) as [Hxy | Hxy].
+  - subst y. repeat rewrite update_eq. auto.
+  - repeat rewrite update_neq; auto.
+Defined.
+
+(* Syntax *)
 Disable Notation "/\".
 Disable Notation "\/".
 Disable Notation "'exists'" (all).
@@ -46,6 +114,7 @@ Notation "( x )" := x (in custom stlc, x at level 99).
 Notation "( x )" := x (in custom stlc_ty, x at level 99).
 Notation "x" := x (in custom stlc at level 0, x constr at level 0).
 Notation "x" := x (in custom stlc_ty at level 0, x constr at level 0).
+Notation "{ x }" := x (in custom stlc at level 1, x constr).
 
 Notation "S -> T"           := (Ty_Arrow S T)
   (in custom stlc_ty at level 50, right associativity).
@@ -60,24 +129,6 @@ Notation "S * T"            := (Ty_Prod S T)
 Notation "'List' T"         := (Ty_List T)
   (in custom stlc_ty at level 0).
 
-Coercion tm_var : INDEX >-> tm.
-Notation "\ x : T , t" := (tm_abs x T t)
-  (in custom stlc at level 90,
-  x at level 99,
-  T custom stlc_ty at level 99,
-  t custom stlc at level 99,
-  left associativity).
-Notation "x y" := (tm_app x y)
-  (in custom stlc at level 1, left associativity).
-Notation "t '.elim' T" := (tm_elim t T)
-  (in custom stlc at level 1).
-Notation "'unit'" := (tm_unit)
-  (in custom stlc at level 0).
-(* omitted *)
-
-Notation "{ x }" := x (in custom stlc at level 1, x constr).
-
-(* Operations *)
 Reserved Notation "'[' x ':=' s ']' t"
   (in custom stlc at level 20, x constr).
 Fixpoint subst (x : INDEX) (e : tm) (t : tm) : tm :=
@@ -112,7 +163,7 @@ Inductive value : tm -> Type :=
   | v_nil T         : value (tm_nil T)
   | v_cons t1 t2    : value t1 -> value t2 -> value (tm_cons t1 t2)
 .
-Global Hint Constructors value : core.
+Hint Constructors value : core.
 
 Reserved Notation "t '-->' t'" (at level 40).
 Inductive step : tm -> tm -> Type :=
@@ -197,15 +248,14 @@ Inductive step : tm -> tm -> Type :=
     value v1 ->
     tm_let x v1 t2 --> <{[x:=v1]t2}>
 where "t '-->' t'" := (step t t').
-Global Hint Constructors step : core.
+Hint Constructors step : core.
 
 Definition context : Type := map ty.
-Definition empty : context := empty.
 Reserved Notation "Gamma '|--' t '\in' T" (at level 40, T custom stlc_ty at level 0).
 Inductive has_type : tm -> ty -> context -> Type :=
-  | T_Var (Gamma : context) (x : INDEX) T : Gamma x = Some T ->
-    Gamma |-- x \in T
-  | T_Abs (Gamma : context) (x : INDEX) T1 T2 t :
+  | T_Var (Gamma : context) x T : Gamma x = Some T ->
+    Gamma |-- tm_var x \in T
+  | T_Abs (Gamma : context) x T1 T2 t :
     (x |-> T1; Gamma) |-- t \in T2 ->
     Gamma |-- tm_abs x T1 t \in (T1 -> T2)
   | T_App (Gamma : context) T1 T2 t1 t2 :
@@ -259,4 +309,148 @@ Inductive has_type : tm -> ty -> context -> Type :=
     (x |-> T1; Gamma) |-- t2 \in T2 ->
     Gamma |-- tm_let x t1 t2 \in T2
 where "Gamma '|--' t '\in' T" := (has_type t T Gamma).
-Global Hint Constructors has_type : core.
+Hint Constructors has_type : core.
+
+
+Lemma weaken t T :
+  forall (G1 : context), G1 |-- t \in T ->
+  forall (G2 : context), includedin G1 G2 ->
+  G2 |-- t \in T.
+Proof.
+  introv HT; induction HT; intros; eauto 7 using includedin_update.
+Defined.
+
+Corollary weaken_empty t T :
+  empty |-- t \in T -> forall G, G |-- t \in T.
+Proof.
+  intros. eapply weaken; eauto. discriminate.
+Defined.
+
+Corollary has_type_extensionality :
+  forall G1 G2 t T,
+  G1 ~ G2 -> G1 |-- t \in T -> G2 |-- t \in T.
+Proof.
+  introv Hext HT. eapply weaken; eauto. congruence.
+Defined.
+
+(* Instance equiv_rel {A} :
+  Equivalence (@mapeq A) :=
+{|
+  Equivalence_Reflexive := mapeq_refl;
+  Equivalence_Symmetric := mapeq_sym;
+  Equivalence_Transitive := mapeq_trans
+|}.
+
+Instance update_morphism {A} x v :
+  CMorphisms.Proper (CMorphisms.respectful (@mapeq A) (@mapeq A)) (update x v) := fun _ _ => mapeq_cong _ _ _ _.
+
+Instance has_type_morphism t T :
+  CMorphisms.Proper (CMorphisms.respectful mapeq iffT) (has_type t T) :=
+  (fun m1 m2 Hequ =>
+   (has_type_extensionality m1 m2 t T Hequ,
+   has_type_extensionality m2 m1 t T (mapeq_sym m1 m2 Hequ))). *)
+
+Theorem progress : forall t T,
+  empty |-- t \in T ->
+  value t \/ exists t', t --> t'.
+Proof.
+  Ltac instantiate_IH :=
+    repeat match goal with
+    | IH : empty = empty -> _ |- _ =>
+      specialize (IH eq_refl);
+      destruct IH as [? | [? ?]]; eauto
+    end.
+  Ltac invert_value :=
+    try match goal with
+    | Hv : value ?t,
+      HT : empty |-- ?t \in _ |- _ =>
+      solve [inverts Hv; inverts HT; eauto]
+    end.
+  intros t T HT. remember empty as Gamma.
+  induction HT; try subst Gamma; eauto;
+  instantiate_IH; invert_value.
+  discriminate.
+Defined.
+
+Theorem subst_type x U v :
+  empty |-- v \in U -> forall t Gamma T,
+  (x |-> U ; Gamma) |-- t \in T ->
+  Gamma |-- <{[x:=v]t}> \in T.
+Proof.
+  Ltac remember_context Gamma :=
+    match goal with
+    | H : has_type ?t ?T Gamma |- ?g =>
+      let H2 := fresh "H" in
+      let p := fresh "p" in
+        assert (H2 : forall (p : context), p ~ Gamma -> has_type t T p -> g); [clear H; intros p Hequ H | eauto]
+    end.
+  Ltac subst_context G :=
+    repeat match goal with
+    | Hequ : G ~ _,
+      Heq : G _ = _ |- _ =>
+      rewrite Hequ in Heq
+    end.
+  Ltac eq_case :=
+    repeat match goal with
+    | |- _ |-- (if ?x =? ?y then _ else _) \in _ =>
+      destruct (eqb_spec x y); subst ; eauto using weaken_empty
+    | H : (?s |-> _ ; _) ?s = Some _ |- _ =>
+      rewrite update_eq in H; inverts H; eauto using weaken_empty
+    | H : (?s |-> _ ; _) ?t = _,
+      H2 : ?s <> ?t |- _ =>
+      rewrite update_neq in H; eauto using weaken_empty
+    | H : (?s |-> _ ; _) ?t = _,
+      H2 : ?t <> ?s |- _ =>
+      rewrite update_neq in H; eauto using weaken_empty
+    end.
+  Ltac enough_cong :=
+    match goal with
+    | H : _ |-- ?t \in ?T |- _ |-- ?t \in ?T =>
+      gen H; eapply has_type_extensionality
+    | H : forall G, _ -> G |-- ?t \in ?T |- _ |-- ?t \in ?T =>
+      apply H
+    end.
+  Ltac subst_cong :=
+    match goal with
+    | Hequ : ?G ~ _ |- ?G ~ _ =>
+      apply (mapeq_trans _ _ _ Hequ)
+    | Hequ : ?G ~ _ |- (_ |-> _; ?G) ~ _ =>
+      apply (mapeq_trans _ _ _ (mapeq_cong _ _ _ _ Hequ))
+    | Hequ : ?G ~ _ |- (_ |-> _; _ |-> _; ?G) ~ _ =>
+      apply (mapeq_trans _ _ _ (mapeq_cong _ _ _ _ (mapeq_cong _ _ _ _ Hequ)))
+    end.
+  introv HTv HT.
+  remember_context (x |-> U ; Gamma); gen Gamma.
+  induction HT;
+  intros Gamma' Heq; subst_context Gamma;
+  simpl; eauto;
+  try econstructor; eauto; eq_case; enough_cong; try subst_cong;
+  eauto using update_shadow, update_permute, mapeq_cong.
+  - (* list ABA=AB *)
+    unfold update. intros z.
+    destruct (x =? z), (y =? z); reflexivity.
+  - (* list ABC=CAB *)
+    eapply mapeq_trans.
+    + eapply mapeq_cong.
+      eapply update_permute; auto.
+    + eapply update_permute; auto.
+Defined.
+
+Theorem preservation t t' T :
+  empty |-- t \in T -> t --> t' -> empty |-- t' \in T.
+Proof.
+  intros HT. remember empty as Gamma. gen t'.
+  induction HT; subst Gamma; try discriminate;
+  introv HS; inverts HS; eauto;
+  try match goal with
+  | H : has_type _ (?c ?T1) _ |- _ =>
+    inverts H
+  | H : has_type _ (?c ?T1 ?T2) _ |- _ =>
+    inverts H
+  end;
+  eauto using subst_type.
+Defined.
+
+End STLC.
+
+Check progress.
